@prefix : <http://ois.vub.ac.be/foodprint/ontology/routes#> .
@prefix geo: <http://www.w3.org/2003/01/geo/wgs84_pos#> .
@prefix owl: <http://www.w3.org/2002/07/owl#> .
@prefix rdf: <http://www.w3.org/1999/02/22-rdf-syntax-ns#> .
@prefix xml: <http://www.w3.org/XML/1998/namespace> .
@prefix xsd: <http://www.w3.org/2001/XMLSchema#> .
@prefix rdfs: <http://www.w3.org/2000/01/rdf-schema#> .
@prefix time: <http://www.w3.org/2006/time#> .
@prefix opengis: <http://www.opengis.net/ont/geosparql#> .
@base <http://ois.vub.ac.be/foodprint/ontology/routes> .

<http://ois.vub.ac.be/foodprint/ontology/routes> 
   rdf:type owl:Ontology ;
   rdfs:label "FoodPrint Routes"@en ;
   rdfs:description  "An ontology for describing the routes a products travels along, with the purpose of deriving a score coined 'FoodPrint' that describes how big the environmental impact of a certain product is"@en .

#################################################################
#    Annotation properties
#################################################################

###  http://swrl.stanford.edu/ontologies/3.3/swrla.owl#isRuleEnabled
<http://swrl.stanford.edu/ontologies/3.3/swrla.owl#isRuleEnabled> rdf:type owl:AnnotationProperty .


#################################################################
#    Object Properties
#################################################################

###  http://ois.vub.ac.be/foodprint#consistsOfConnections
:consistsOfConnections rdf:type owl:ObjectProperty ;
                       rdfs:domain :Route ;
                       rdfs:range :Connection ;
                       rdfs:label "route consists of connections"@en ;
                       rdfs:comment "Defines a connection between two distribution points to be part of a route"@en .


###  http://ois.vub.ac.be/foodprint#fromPoint
:fromPoint rdf:type owl:ObjectProperty ,
                    owl:FunctionalProperty ;
           rdfs:domain :Edge ;
           rdfs:range :DistributionPoint ;
           rdfs:label "from point"@en ;
           rdfs:comment "Vertex a in a directed edge a -> b"@en .


###  http://ois.vub.ac.be/foodprint#location
:location rdf:type owl:ObjectProperty ;
          rdfs:domain :DistributionPoint ;
          rdfs:range geo:Point ;
          rdfs:label "location"@en ; 
          rdfs:comment "The location of a distribution point"@en.

###  http://ois.vub.ac.be/foodprint#ofRoute
:ofRoute rdf:type owl:ObjectProperty ;
         rdfs:domain :Reachable ;
         rdfs:range :Route ;
         rdfs:label "of route"@en ;
         rdfs:comment "The route reachable edge belongs to"@en.

:hasReachable rdf:type owl:ObjectProperty ;
              owl:inverseOf :ofRoute ;
              rdfs:label "hasReachable"@en ;
              rdfs:comment "The route has some reachable edges, that can be used to validate the route"@en .


###  http://ois.vub.ac.be/foodprint#routeHasEndpoint
:routeHasEndpoint rdf:type owl:ObjectProperty ,
                           owl:FunctionalProperty ;
                  rdfs:domain :Route ;
                  rdfs:range :Shop ;
                  rdfs:label "route has endpoint"@en ;
                  rdfs:comment "Denotes that the given route has the given shop as an endpoint" .


###  http://ois.vub.ac.be/foodprint#routeHasStartpoint
:routeHasStartpoint rdf:type owl:ObjectProperty ;
                    rdfs:subPropertyOf owl:topObjectProperty ;
                    rdf:type owl:FunctionalProperty ;
                    rdfs:domain :Route ;
                    rdfs:range :DistributionPoint ;
                    rdfs:label "route has starting point"@en ; 
                    rdfs:comment "Denotes that the given route has the given distribution point at its origin" . 


###  http://ois.vub.ac.be/foodprint#toPoint
:toPoint rdf:type owl:ObjectProperty ,
                  owl:FunctionalProperty ;
         rdfs:domain :Edge ;
         rdfs:range :DistributionPoint ;
         rdfs:label "to point"@en ;
         rdfs:comment "Vertex b in a direct edge a -> b"@en .


###  http://ois.vub.ac.be/foodprint#transportedBy
:transportedBy rdf:type owl:ObjectProperty ,
                        owl:FunctionalProperty ;
               rdfs:domain :Connection ;
               rdfs:range :TransportMode ;
               rdfs:label "transported by"@en ;
               rdfs:comment "A connection has a transport mode, this means that the given transport is used for transporting the product across the given route"@en .


###  http://ois.vub.ac.be/foodprint#travelsAlong
:travelsAlong rdf:type owl:ObjectProperty ;
              rdfs:domain :Product ;
              rdfs:range :Route ;
              rdfs:label "travels along"@en ;
              rdfs:comment "A product can be transported over multiple routes"@en .


#################################################################
#    Data properties
#################################################################

###  http://ois.vub.ac.be/foodprint#footprintPerKm
:footprintPerKm rdf:type owl:DatatypeProperty ;
                rdfs:domain :TransportMode ;
                rdfs:range xsd:int ;
                rdfs:label "foodprint per km" ;
                rdfs:comment "Denotes the amount of CO2 that is emitted for each kilometer to mode of transport travels" .


:locationWkt   rdf:type owl:DatatypeProperty ;
               rdfs:domain :DistributionPoint ;
               rdfs:range opengis:wktLiteral ;
               rdfs:label "locationWkt" ;
               rdfs:comment "Denotes the location as WKT (Well Known Text Format) for representing points (eg. POINT(latitude, longitude)" .

#################################################################
#    Classes
#################################################################

###  http://ois.vub.ac.be/foodprint#Connection
:Connection rdf:type owl:Class ;
            rdfs:subClassOf :Edge ;
            rdfs:label "Connection"@en ; 
            rdfs:comment "A connection between two distribution points"@en .



###  http://ois.vub.ac.be/foodprint#DistributionPoint
:DistributionPoint rdf:type owl:Class ;
                   rdfs:label "Distribution Point" ;
                   rdfs:comment "A distribution point from which a product can come from, or can travel along" .
      


###  http://ois.vub.ac.be/foodprint#Edge
:Edge rdf:type owl:Class ;
      rdfs:label "Edge"@en ;
      rdfs:comment """
      An edge between two distribution points. This is an abstraction of the Connection, which allows 
      other kinds of edge to be produced between distributionpoints
      """@en .

###  http://ois.vub.ac.be/foodprint#Reachable
:Reachable rdf:type owl:Class ;
           rdfs:subClassOf :Edge ;
           rdfs:label "Reachable"@en ;
           rdfs:comment "Is an edge that denotes that a point b is reachable from a point a"@en .

##  http://ois.vub.ac.be/foodprint#Route
:Route rdf:type owl:Class ;
       rdfs:label "Route"@en ;
       rdfs:comment "A route consists of connection, connecting multiple distirbution points together"@en .


###  http://ois.vub.ac.be/foodprint#Shop
:Shop rdf:type owl:Class ;
      rdfs:subClassOf :DistributionPoint ;
      rdfs:label "Shop"@en ;
      rdfs:comment "A shop is the last distribution point is a route. It is where the user can find their products"@en .

###  http://ois.vub.ac.be/foodprint#TransportMode
:TransportMode rdf:type owl:Class ;
               rdfs:label "Transport Mode" @en ;
               rdfs:comment "The mode of transport, eg. car, plane, boat, ..." .

###  http://www.w3.org/2003/01/geo/wgs84_pos#Point
geo:Point rdf:type owl:Class .


### http://ois.vub.ac.be/foodprint/routes#Product
:Product rdf:type owl:Class ;
         rdfs:label "Product"@en ;
         rdfs:comment "A product that can travel along a round"@en .

#################################################################
#    Individuals
#################################################################


#################################################################
#    General axioms
#################################################################



[ rdf:type owl:AllDisjointClasses ;
  owl:members ( :Connection
                :Route
                :Shop
                :TransportMode
              )
] .


#################################################################
#    Rules
#################################################################

